theories/OptionNotations.v
@@ -1,0 +1,6 @@
+(* Define only as a notation becaues Function can't see through otherwise *)
+Notation "'do' x ← e0 ; e1" :=
+  (match e0 with
+   | Some x => e1
+   | _ => None
+   end) (x pattern, at level 200, left associativity).
